before cleanup

Leanegraph/core/Naive.lean
@@ -1,15 +1,14 @@
-import Batteries.Data.UnionFind
-
+import Leanegraph.core.SharedDefs
+import Leanegraph.core.Helpers
+import Leanegraph.core.Hashcons
 
 /-
   Implementations of E-Node, E-Class, E-Graph and functions that operate on them
 -/
 variable {α : Type _} [DecidableEq α] [Hashable α] [Repr α]
-variable {D : Type _} [BEq D] [Inhabited D]
+variable {D : Type _} [DecidableEq D] [Inhabited D]
 
 namespace Naive
-
-abbrev EClassId := Nat
 
 
 structure ENode (α : Type _ ) where
@@ -29,14 +28,65 @@ deriving Repr
     E-class Map M - Map of *e-class ids to e-classes*
     Hashcons H - Map of *e-nodes to e-class ids*
 -/
-structure EGraph (α : Type _) (D : Type _) [DecidableEq α] [Hashable α] where
-  uf    : Batteries.UnionFind
-  ecmap : List <| EClassId × (EClass α D)
-  hcons : List <| ENode α × EClassId -- TODO: does this make it less readable?
-  dirty : List <| EClassId × ENode α  -- hegg's version, keeps 2
-  aldrt : List <| EClassId × ENode α
-  opmap : List <| α × (List EClassId)
 
+structure EGraph (α : Type _) (D : Type _) [DecidableEq α] [Hashable α] where
+  uf    : UF -- def UF := List <| EClassId × EClassId
+  ecmap : List <| EClassId × (EClass α D)
+  hcons : List <| ENode α × EClassId
+  dirty : List EClassId
+  aldrt : List EClassId
+/-
+def ufFind (eg : EGraph α D) (id : EClassId) : EClassId :=
+  eg.uf.lookup id |>.getD id
+
+def ufUnion (eg : EGraph α D)  (id₁ id₂ : EClassId) : EGraph α D :=
+  let leader₁ := ufFind eg id₁
+  let leader₂ := ufFind eg id₂
+  let newUf := eg.uf.map (λ (member, leader) =>
+    if leader == leader₂ then (member, leader₁) else (member, leader)
+  )
+  {eg with uf := newUf}
+-/
+
+def ecmapLookup (eg : EGraph α D) : EClassId → Option (EClass α D) :=
+  λ id => eg.ecmap.lookup id
+
+def hcLookup (eg : EGraph α D) : ENode α → Option EClassId :=
+  λ en => eg.hcons.lookup en
+
+-- def insertHCons (hc : List <| ENode α × EClassId) (k : ENode α) (v : EClassId) : List <| ENode α × EClassId :=
+--   (k, v) :: hc.filter (λ p => p.1 != k)
+def insertHCons (hc : List <| ENode α × EClassId) (k : ENode α) (v : EClassId) : List <| ENode α × EClassId :=
+  uniqueInsert hc k v
+
+def insertECMap (ec : List <| EClassId × EClass α D) (k : EClassId) (v : EClass α D) : List <| EClassId × EClass α D :=
+  uniqueInsert ec k v
+
+-- #eval List.filter (λ x => x ≠ 3) [1,2,3,4,5]
+
+def EGraph.size (eg : EGraph α D) : Nat :=
+  List.length eg.uf
+
+def numCanonClasses (eg : EGraph α D) : Nat :=
+  eg.uf.filter (λ (id, cid) => id == cid) |>.length
+
+def numClasses (eg : EGraph α D) : Nat :=
+  eg.uf.map Prod.snd |>.eraseDups |>.length
+/-
+theorem theTwoFunctionsAboveAreEqual (eg : EGraph α D) (h : UF.pairCanon eg.uf)
+  : numCanonClasses eg = numClasses eg := by
+  unfold numCanonClasses numClasses
+  unfold UF.pairCanon at h
+  simp[]
+  suffices h :
+    (eg.uf.filter (fun x => x.fst == x.snd)).map Prod.fst = (eg.uf.map Prod.snd).eraseDups
+    by
+      simp[Eq.symm h]
+
+  apply List.ext_getElem
+
+  sorry
+-/
 
 instance [Inhabited α] : Inhabited (ENode α) where
   default := {
@@ -88,19 +138,19 @@ def EClass.fromNode {α : Type _} (en : ENode α) (data : D) : EClass α D :=
   }
 
 
-def EClass.merge (ec₁ ec₂ : EClass α D) (join : D → D → D) : EClass α D:=
+def EClass.merge [Analysis α D] (ec₁ ec₂ : EClass α D) : EClass α D:=
   {
-    nodes :=  ec₁.nodes.append ec₂.nodes |>.eraseDups
-    parents := ec₁.parents ++ ec₂.parents
-    data := join (ec₁.data) (ec₂.data)
+    nodes :=  ec₁.nodes.append ec₂.nodes-- |>.eraseDups
+    parents := ec₁.parents ++ ec₂.parents-- |>.eraseDups
+    data := Analysis.join (α := α) (D := D) (ec₁.data) (ec₂.data)
   }
-
 
 def updateEClassParents (en : ENode α) (eid : EClassId) (cur : EClassId × EClass α D) : EClassId × EClass α D :=
   (cur.1, ec) where
     parent := (en, eid)
     ec     := {cur.2 with parents := parent :: cur.2.parents}
 
+/-
 def updateParents (ecmap : List <| EClassId × EClass α D) (en : ENode α) (eid : EClassId)
   : List <| EClassId × (EClass α D) :=
   ecmap.map
@@ -110,40 +160,80 @@ def updateParents (ecmap : List <| EClassId × EClass α D) (en : ENode α) (eid
       else
         el
     )
+-/
+def updateParents (ecmap : List <| EClassId × EClass α D) (en : ENode α) (eid : EClassId)
+  : List <| EClassId × (EClass α D) :=
+  en.args.foldl (λ acc argId =>
+    match acc.lookup argId with
+    | some ec =>
+        let updatedEc := { ec with parents := (en, eid) :: ec.parents }
+        insertECMap acc argId updatedEc
+    | none => acc
+  ) ecmap
 
-def EGraph.size (eg : EGraph α D) : Nat :=
-  eg.uf.size
 
 def EGraph.empty : EGraph α D:=
   {
-    uf    := Batteries.UnionFind.empty
+    uf    := []
     ecmap := []
     hcons := []
     dirty := []
     aldrt := []
-    opmap := []
   }
 
 abbrev EGraphM (α : Type _) (D : Type _) [DecidableEq α] [Hashable α] := StateM (EGraph α D)
-
+/-
 def lookupCanonicalEClassId (id : EClassId) : EGraphM α D <| EClassId := do
   let eg ← get
-  let ⟨uf', res⟩ := eg.uf.find! id
+  let ⟨uf', res⟩ := eg.uf.ufFind id
   let _ ← set { eg with uf := uf' }
   return res
-
-def canonicalise (en : ENode α) : EGraphM α D (ENode α) := do
-  let newargs : List EClassId ← en.args.mapM lookupCanonicalEClassId
-  return { en with args := newargs}
-
-def findClass (en : ENode α) : EGraphM α D (Option EClassId) := do
-  let en' ← canonicalise en
+-/
+def lookupCanonicalEClassId (eg : EGraph α D) (id : EClassId) : EClassId :=
+  eg.uf.find id
+/-
+def lookupCanonicalEClassIdM (id : EClassId) : EGraphM α D <| EClassId := do
   let eg ← get
-  match eg.hcons.lookup en' with
+  return eg.uf.find id
+
+def canonicaliseM (en : ENode α) : EGraphM α D (ENode α) := do
+  let newargs : List EClassId ← en.args.mapM lookupCanonicalEClassIdM
+  return { en with args := newargs}
+-/
+def canonicalise (eg : EGraph α D) (en : ENode α) : ENode α :=
+  {en with args := en.args.map (lookupCanonicalEClassId eg)}
+/-
+def betterCanonicaliseM? (en : ENode α) : EGraphM α D (ENode α) := do
+  let eg ← get
+  return canonicalise eg en
+-/
+
+
+/-
+  Calls:
+    - Canonicalise
+  Called By:
+    - Push (node canonicalised before call, no need to canon it again)
+  Do we need to lookupCanonicalEClassId the hcons lookup?
+  In the naive, the hcons should always be canon
+-/
+def findClassM (en : ENode α) : EGraphM α D (Option EClassId) := do
+  -- let en' ← canonicalise en
+  let eg ← get
+  /-
+  match eg.hcons.lookup en with
   | some eClassId =>
     return some eClassId
   | none =>
     return none
+  -/
+  -- return eg.hcons.lookup en
+  return hcLookup eg en
+
+
+def findClass (eg : EGraph α D) (en : ENode α) : Option EClassId :=
+  hcLookup eg en
+
 
 /-
   Adds a node to the egraph
@@ -151,206 +241,258 @@ def findClass (en : ENode α) : EGraphM α D (Option EClassId) := do
   If it doesn't, add it to the UF, E-Class Map, HCons
   Returns the new ID (which is the size of the E-Graph)
 -/
-def push {D : Type _} [Inhabited (EClass α D)] [Inhabited D] (en : ENode α) (make : ENode α → List D → D): EGraphM α D (EClassId) := do
-  let en' ← canonicalise en
-  match ← findClass en' with
-  | some ecId =>
-    return ecId
+
+
+def push [Analysis α D] (eg : EGraph α D) (en : ENode α) : EGraph α D × EClassId :=
+  let en' := canonicalise eg en
+  match hcLookup eg en' with
+  | some id => (eg, id)
   | none =>
-    let eg ← get
-    let curSize := eg.size
-    let ecmap' := updateParents eg.ecmap en' curSize
+    let (newUf, curSize) := eg.uf.push
+    let ecmap'  := updateParents eg.ecmap en' curSize
     let childData := en'.args.map (λ id =>
-      ((eg.ecmap.lookup id).getD EClass.empty).data
+      ((ecmapLookup eg id).getD EClass.empty).data
+      -- technically says even if doesn't exist in ecmap we are fine?
+      -- so should not do that
     )
+    let ecmap'' := insertECMap ecmap' curSize (EClass.fromNode en' (Analysis.make en' childData))
+    let hcons'  := insertHCons eg.hcons en' curSize
 
+    (Analysis.modify {eg with
+      uf := newUf,
+      ecmap := ecmap'',
+      hcons := hcons',
+      dirty := curSize :: eg.dirty,
+      aldrt := curSize :: eg.aldrt
+    } curSize, curSize)
 
-    let ecmap'' := (curSize, (EClass.fromNode en' (make en' childData))) :: ecmap'
-    let hcons' := eg.hcons.insert (en', curSize)
-
-    let curList := (eg.opmap.lookup en'.head).getD []
-    set { eg with
-            uf := eg.uf.push,
-            ecmap := ecmap'',
-            hcons := hcons',
-            opmap := (en'.head, curSize :: curList) :: eg.opmap
-            dirty := (curSize, en') :: eg.dirty
-            aldrt := (curSize, en') :: eg.aldrt
-        }
-    return curSize
-
--- I never use the return value here but hegg (haskell egg) returns eclassid, keep that for now
--- Similar question to the above, are we bound to a do-block because of the union-find here?
--- Do do-blocks make it harder to prove anything?
--- TODO: do i have to ensure the invariant holds before and after?
--- https://hackage-content.haskell.org/package/hegg-0.6.0.0/docs/src/Data.Equality.Graph.html#merge
--- TODO: i think we can extract a lot of these into smaller pure helper functions
--- the merge eclasses, hashcons
-def union (id₁ id₂ : EClassId) (join : D → D → D) : EGraphM α D (EClassId) := do
+def union [Analysis α D] (eg : EGraph α D) (id₁ id₂ : EClassId) : EGraph α D × EClassId :=
 
   -- Get canonical classes for the inputs
-  let id₁' ← lookupCanonicalEClassId id₁
-  let id₂' ← lookupCanonicalEClassId id₂
+  let id₁' := lookupCanonicalEClassId eg id₁
+  let id₂' := lookupCanonicalEClassId eg id₂
   -- In same class, nothing more to do
   if id₁' = id₂' then
-    return id₁'
+    (eg, id₁')
   -- In different class, we do work
   else
-    -- moved this here for less operations?
-    let eg ← get
     -- Update union find
-    let uf' := eg.uf.union! id₁' id₂'
-    let (uf''', leaderClassId) := uf'.find! id₁'
-    -- more path compression........?
-    let (uf'',  _) := uf'''.find! id₂'
-    -- Update EClass, EClassMap and Hashcons with new UF canonies
-    let fromId := if id₁' = leaderClassId then id₂' else id₁'
-    -- merge std hashmap union
-    -- also touch parents -- not in egg style deferred
-    let lCls := (eg.ecmap.lookup leaderClassId).getD EClass.empty
-    let sCls := (eg.ecmap.lookup fromId).getD EClass.empty
-    let mergedClass := EClass.merge lCls sCls join
+    let (uf', leaderClassId) := eg.uf.union id₁' id₂'
+    -- Technically leader is always id₁' here
+    -- but for readability we keep the names
+    let toId := id₁'
+    let frId := id₂'
 
-    let newEcmap := (leaderClassId, mergedClass) :: eg.ecmap.filter (λ (id, _) => id ≠ fromId && id ≠ leaderClassId)
+    let lCls := (eg.ecmap.lookup toId).getD EClass.empty
+    let sCls := (eg.ecmap.lookup frId).getD EClass.empty
 
-    let newDirty := (sCls.parents.map Prod.swap) ++ eg.dirty
+    let newEClass := EClass.merge lCls sCls
 
-    let newData := join lCls.data sCls.data
-    let nAnlDrt :=
-      (if newData != sCls.data then (sCls.parents.map Prod.swap) else [])
+    -- let ecmap'    := uniqueInsert (uniqueRemove eg.ecmap frId) leaderClassId newEClass
+
+    -- Insert new leader class
+    let ecmap'    := uniqueInsert eg.ecmap leaderClassId newEClass
+    -- Replace old follower class with empty class for.... idk reasons (leave alone because I don't think deleting is good in array later)
+    let ecmap''   := uniqueInsert   ecmap' frId          EClass.empty
+
+    let newData   := newEClass.data
+    let newDirty  := leaderClassId :: eg.dirty
+    let newAldrt  :=
+      (if newData != sCls.data then [leaderClassId] else [])
       ++
-      (if newData != lCls.data then (lCls.parents.map Prod.swap) else [])
+      (if newData != lCls.data then [leaderClassId] else [])
       ++
       eg.aldrt
 
-    let _ ← set {
-                  eg with
-                  uf := uf''
-                  ecmap := newEcmap
-                  dirty := newDirty
-                  aldrt := nAnlDrt
-                }
-    return leaderClassId
+    let eg' := {
+      eg with
+      uf    := uf',
+      ecmap := ecmap'',
+      dirty := newDirty,
+      aldrt := newAldrt
+    }
+
+    (Analysis.modify eg' leaderClassId, leaderClassId)
+
+def unionReduces : sorry := sorry
 
 
+def repairAnalysis [Analysis α D] (eg : EGraph α D) (id : EClassId) : EGraph α D :=
+  let canonId := lookupCanonicalEClassId eg id
 
-
-
-def rebuildOpMap : EGraphM α D Unit := do
-  let eg ← get
-
-  let newOpMap := eg.ecmap.foldl (λ opmap (id, eclass) =>
-    eclass.nodes.foldl (λ opmap node =>
-      let cur := (opmap.lookup node.head).getD []
-      (node.head, id :: cur) :: opmap.filter (λ a => a.1 ≠ node.head)
-    ) opmap
-  ) []
-
-  set { eg with opmap := newOpMap}
-
-/-
-  for (id, eclass) in eg.ecmap do
-    for node in eclass.nodes do
-      let head := node.head
-      let currentArr := newOpMap.getD head []
-      newOpMap := newOpMap.insert head (currentArr.push id)
--/
-  set { eg with opmap := newOpMap }
-
-
-
-def repairHegg (id : EClassId) (en : ENode α) [Analysis α D] : EGraphM α D <| Unit := do
-  let eg ← get
-  match eg.hcons.lookup en with
-  | none =>
-    let _ ← set {eg with hcons := eg.hcons.insert (en, id)}
-  | some existing =>
-    let _ ← set {eg with hcons := eg.hcons.insert (en, id)}
-    let _ ← union existing id (Analysis.join (α := α) (D := D))
-
-def repairAnalysisHegg (id : EClassId) (en : ENode α) [Analysis α D] : EGraphM α D <| Unit := do
-  let eg ← get
-  match eg.ecmap.lookup id with
-  | none => return ()
+  match eg.ecmap.lookup canonId with
+  | none => eg
   | some cls =>
-    let childData := en.args.map λ argId =>
-      ((eg.ecmap.lookup argId).getD EClass.empty).data
-    let newData := Analysis.join (α := α) (D:= D) cls.data (Analysis.make en childData)
-    if newData != cls.data then
-      let cls'     := {cls with data := newData}
-      let newAldrt := cls.parents.map Prod.swap ++ eg.aldrt
-      let eg'      := {eg with
-                        ecmap := (id, cls') :: eg.ecmap.filter (λ ec => ec.1 != id)
-                        aldrt := newAldrt
-                      }
-      let _ ← set (Analysis.modify eg' id)
+    let newData := cls.nodes.map (λ en =>
+      let canonArgs := en.args.map (lookupCanonicalEClassId eg)
+      let childData := canonArgs.map (λ argId =>
+        ((eg.ecmap.lookup argId).getD EClass.empty).data
+      )
+      Analysis.make en childData
+    )
 
--- def repairAnalysisHegg ()
+    let joinData := newData.foldl (Analysis.join (α := α) (D := D)) cls.data
 
-partial def rebuildHegg [Analysis α D] : EGraphM α D <| Unit := do
-  let eg ← get
-  if eg.dirty.isEmpty && eg.aldrt.isEmpty then return()
+    if joinData ≠ cls.data then
+      let cls' := { cls with data := joinData}
+      let parentIds := cls.parents.map Prod.snd
+      let eg' := { eg with
+        ecmap := insertECMap eg.ecmap canonId cls',
+        aldrt := parentIds ++ eg.aldrt
+      }
 
-  let emptyEgr := {eg with dirty := [], aldrt := []}
-  let _ ← set emptyEgr
-
-  let findEmpty := λ id => emptyEgr.uf.find! id |>.2
+      Analysis.modify eg' canonId
+    else eg
 
 
+def repair (eg : EGraph α D) (id : EClassId) : EGraph α D × List (EClassId × EClassId) :=
+  let canonId := lookupCanonicalEClassId eg id
 
-  let wl := eg.dirty.map (λ p =>
-                (findEmpty p.1, {p.2 with args := p.2.args.map findEmpty})
-              ) |>.eraseDups
+  match ecmapLookup eg canonId with
+  | none => (eg, []) --
+  | some eCls =>
+
+    let (updateHCons, collisions) := eCls.parents.foldl (init := (eg.hcons, [])) (λ (hcons', collisions') (node, pId) =>
+      let canonNode := canonicalise eg node
+      let canonId  := eg.uf.find pId
+      let det      := hcons'.filter (λ hc => hc.1 ≠ node)
+      match det.lookup canonNode with
+      | some key => (det, (canonId, key) :: collisions')
+      | none     => ((canonNode, canonId) :: det, collisions')
+    )
+
+    let eg' := {eg with hcons := updateHCons}
 
 
-  wl.forM (λ p => repairHegg p.1 p.2)
 
-  let eg' ← get
-  let findEmpty' := λ id => eg'.uf.find! id |>.2
-  let naldrt := eg.aldrt.map (λ p : EClassId × ENode α =>
-    (findEmpty' p.1, {p.2 with args := p.2.args.map findEmpty'})) |>.eraseDups
 
-  naldrt.forM (λ p => repairAnalysisHegg p.1 p.2)
 
-  rebuildHegg
+    -- Loop 2...
+    let (_, pc) := eCls.parents.foldl (init := ([], [])) (λ (seen, pc) (p : (ENode α × EClassId)) =>
+      let canon := canonicalise eg' p.1
+      let canonId := lookupCanonicalEClassId eg' p.2
+      match seen.lookup canon with
+      | some eid => (seen, (eid, canonId) :: pc)
+      | none     => ((canon, canonId) :: seen, pc)
+    )
 
+    let newNodes := eCls.nodes.foldl (init := []) (λ newN en =>
+      let canonN := canonicalise eg' en -- or eg'?
+      -- if newN.any (λ a => a == canonN) then newN else canonN :: newN
+      if newN.contains canonN then newN else canonN :: newN
+    )
+
+    let newParents := eCls.parents.foldl (init := []) (λ newP (en, eid) =>
+      let canonN  := canonicalise eg' en
+      let canonId := lookupCanonicalEClassId eg eid
+      if newP.any (λ (an, ac) => an == canonN && ac == canonId) then newP else (canonN, canonId) :: newP
+    )
+
+    let eg'' := { eg' with
+      ecmap := insertECMap eg'.ecmap canonId {eCls with
+        nodes := newNodes, parents := newParents
+      }
+    }
+
+    (eg'', collisions ++ pc)
+
+
+def rebuildTerminationBy (eg : EGraph α D) : Nat × Nat :=
+  let work := eg.dirty.length + eg.aldrt.length
+  let classes := numCanonClasses eg
+  (classes, work)
+
+def rebuild [Analysis α D] (eg : EGraph α D) : EGraph α D :=
+  if eg.dirty.isEmpty && eg.aldrt.isEmpty then eg
+  else
+    let todo := eg.dirty.map (lookupCanonicalEClassId eg) |>.eraseDups
+    let eg'  := {eg with dirty := []}
+
+    -- Pass through dirty (congruence repair)
+    let eg'' := todo.foldl (λ eg₁ id =>
+      let (eg₂, collisions) := repair eg₁ id
+      collisions.foldl (λ acc (id₁, id₂) =>
+        (union acc id₁ id₂).1) eg₂
+      ) eg'
+    -- Pass through aldrt (uh... analysis repair?)
+    let atodo := eg''.aldrt.map (lookupCanonicalEClassId eg'') |>.eraseDups
+    let eg₃   := { eg'' with aldrt := [] }
+    let eg₄   := atodo.foldl repairAnalysis eg₃
+
+    rebuild eg₄
+termination_by (numClasses eg, eg.dirty.length + eg.aldrt.length)
+decreasing_by
+  simp_wf
+
+  sorry
+
+-- https://leanprover-community.github.io/extras/well_founded_recursion.html
+-- Bottom of the page has example on Nat × Nat
+
+-- TODO: study:
+-- https://web.archive.org/web/20250618125453/https://lean-lang.org/blog/2024-1-11-recursive-definitions-in-lean/
+-- https://www.joachim-breitner.de/blog/817-F91_in_Lean
+-- https://notch1p.xyz/fixpoint-comb (translate)
 /-
-partial def rebuildHegg : EGraphM α D <| Unit := do
-  let eg ← get
-  if eg.dirty.isEmpty then return()
+termination_by λ eg : EGraph α D => rebuildTerminationBy eg
+decreasing_by
+  simp
 
-  let emptiedEgr := EGOps.emptyDirty eg
-  let _ ← set emptiedEgr
-
-  let wl := EGOps.dedupDirty <| EGOps.mapDirty
-              (λ (id, node) =>
-                (
-                  EGOps.findEmpty emptiedEgr id,
-                  EGOps.setArgs node (EGOps.mapArgs (EGOps.findEmpty emptiedEgr) (EGOps.getArgs node))
-              ))
-            (EGOps.getDirty eg)
-
-  EGOps.forMDirty wl fun (id, node) => repairHegg id node
-
-  rebuildHegg
-
+  sorry
 -/
 /-
   For Testing And Execution
   TODO: macros
 -/
-
+/-
 def pushRun [Analysis α D] (en : ENode α) : EGraphM α D EClassId := do
   let id ← push en Analysis.make
-  rebuildHegg
   return id
 
 def unionRun [Analysis α D] (id₁ id₂ : EClassId) : EGraphM α D EClassId := do
-  let id ← union id₁ id₂ (Analysis.join (α := α) (D := D))
-  rebuildHegg
+  let id ← union id₁ id₂
+  return id
+-/
+
+/-
+  Props that might be needed eventually?
+-/
+
+
+
+
+/-
+  Exports for outside use
+-/
+
+def lookupCanonicalEClassIdM (id : EClassId) : EGraphM α D EClassId := do
+  return lookupCanonicalEClassId (← get) id
+
+def pushM [Analysis α D] (en : ENode α) : EGraphM α D EClassId := do
+  let (eg', id) := push (← get) en
+  discard <| set eg'
   return id
 
-def rebuildRun [Analysis α D] : EGraphM α D (Unit) := do
-  rebuildHegg
+def unionM [Analysis α D] (id₁ id₂ : EClassId) : EGraphM α D EClassId := do
+  let (eg', leader) := union (← get) id₁ id₂
+  set eg'
+  return leader
+
+def rebuildM [Analysis α D] : EGraphM α D Unit := do
+  set (rebuild (← get))
+
+
+
+
+
+/-
+  ecmap : List <| EClassId × (EClass α D)
+  hcons : List <| ENode α × EClassId
+  dirty : List EClassId
+  aldrt : List <| EClassId × ENode α
+-/
+
+
+
 
 end Naive
