Leanegraph/core/Hashcons.lean
@@ -1,0 +1,62 @@
+import Leanegraph.core.SharedDefs
+
+namespace Naive
+/-
+  Notes: HCons must always be canonical nodes for lookup purposes, scan code for that also TODO:
+  Also that the UF always points to canonical values
+  Also that the Hcons are unique
+  Make them Prop s?
+  Many things are unique keys, since they're maps
+  Use hcons.insertUnique or something where I define it?
+-/
+/-
+  Basic Union Find, to make it as simple as possible
+  Goals: Reasoning...? Provability...? Not-break-my-head-ability? Pure?
+  Should not be difficult to swap out later
+
+  Some notes
+
+  1. Every ID must have been pushed before use (doable)
+  2. Uf.push must be the only way to add things in (is doable)
+  3. Nothing must be removed, ever (see note 1)
+
+  For 2, note that union only updates and doesn't add/remove classes
+-/
+abbrev UF := List <| EClassId × EClassId
+
+def UF.find (uf : UF) (id : EClassId) : EClassId :=
+  uf.lookup id |>.getD id
+
+-- Leader is always id₁
+def UF.union (uf : UF)  (id₁ id₂ : EClassId) : UF × EClassId:=
+  let leader₁ := uf.find id₁
+  let leader₂ := uf.find id₂
+  if leader₁ == leader₂ then (uf, leader₁)
+  else
+  let newUf := uf.map (λ (member, leader) =>
+    if leader == leader₂ then (member, leader₁) else (member, leader)
+  )
+  (newUf, leader₁)
+
+def UF.size (uf : UF) : Nat :=
+  uf.length
+
+def UF.push (uf : UF) : UF × EClassId :=
+  let newClass := uf.size
+  ((newClass, newClass) :: uf, newClass)
+
+
+-- #eval UF.union (UF.push ([] : UF) |>.1 |> UF.push |>.1 |> UF.push |>.1) 0 2 |>.1
+
+def UF.isValidID (uf : UF) (id : EClassId) : Prop :=
+  id < uf.size
+
+-- because of this, changed def to abbrev
+-- alternatively could define membership for uf but this seems easier?
+-- TODO: abbrev vs def
+def UF.pairCanon (uf : UF) : Prop :=
+  ∀ id cid, (id, cid) ∈ uf → uf.find cid = cid
+
+
+
+end Naive
