Leanegraph/core/examples.lean
@@ -1,0 +1,39 @@
+def search {α} (f : Nat → Option α) (start : Nat) : Option α :=
+  match f start with
+  | .some x => .some x
+  | .none =>
+    match start with
+    | 0 => .none
+    | n+1 => search f n
+
+theorem search_const_none {α} (start : Nat) :
+      search (α := α) (fun _ => .none) start = .none := by
+  induction start with
+  | zero =>
+    rw[search]
+  | succ n ih =>
+    simp[search]
+    exact ih
+
+example : search (fun n => if n * n ≤ 121 then .some n else .none) 100 = .some 11 := by
+  simp[search]
+
+
+def sub2 : Nat → Nat
+| 0 => 0
+| 1 => 0
+| x + 2 => x
+
+#print sub2
+
+example (n : Nat) : sub2 n = n - 2 := by
+ unfold sub2
+ cases n
+ case zero => simp
+ case succ n => grind
+
+
+def search2 {α} (f : Nat → Option α) (start : Nat) : α :=
+  match f start with
+  | .some x => x
+  | .none => search f (start + 1)
